examples/lib/list.v
@@ -1,0 +1,23 @@
+From Stdlib Require Import List String ZArith.
+From shift_reset.lib Require sum.
+From shift_reset.core Require Import syntax syntax_notation.
+From shift_reset.interpreter Require Import interpreter error.
+Import ListNotations.
+
+Local Open Scope term_scope.
+
+Fixpoint int_list_to_val_term (xs : list Z) : val_term :=
+  match xs with
+  | [] => <{ Inl () }>
+  | x :: xs' => <{ Inr ({TVInt x}, {int_list_to_val_term xs'}) }>
+  end.
+
+Fixpoint val_to_int_list (v : val) : exn + list Z :=
+  match v with
+  | VInl VTt => inr []
+  | VInr (VPair (VInt x) v') => sum.map (cons x) (val_to_int_list v')
+  | _ => inl (Failure "val_to_int_list")
+  end.
+
+Definition eval_term_to_int_list (fuel : nat) (t : term) : exn + list Z :=
+  sum.bind (eval_term fuel t) val_to_int_list.
